WIP

theories/Eq/UpToTaus.v
@@ -35,7 +35,7 @@
  *)
 
 (* begin hide *)
-Require Import Paco.paco.
+Require Import Paco.paco Program Setoid Morphisms RelationClasses.
 
 From ITree Require Import
      Core.ITreeDefinition
@@ -45,9 +45,156 @@ Import ITreeNotations.
 Local Open Scope itree.
 (* end hide *)
 
+Require Import Classical.
+Section EUTT_inftaus.
+
+Context {E : Type -> Type}.
+
+Definition notauF {R} (t : itree' E R) : Prop :=
+  match t with
+  | TauF _ => False
+  | _ => True
+  end.
+Hint Unfold notauF.
+
+Notation notau t := (notauF (observe t)).
+
+Inductive untausF {R} :
+  itreeF E R (itree E R) -> itreeF E R (itree E R) -> Prop :=
+| NoTau ot0 : untausF ot0 ot0
+| OneTau ot t' ot0 (OBS: TauF t' = ot) (TAUS: untausF (observe t') ot0): untausF ot ot0
+.
+Hint Constructors untausF.
+
+Definition unalltausF {R} ot ot0 := untausF ot ot0 /\ @notauF R ot0.
+Hint Unfold unalltausF.
+
+Notation unalltaus t t' := (unalltausF (observe t) (observe t')).
+
+Inductive taus_one {R} (P: itree E R -> Prop) : itree' E R -> Prop :=
+| to_step t (BASE: P t) : taus_one P (TauF t)
+.
+Hint Constructors taus_one.
+
+Definition inftaus_ {R} P t := @taus_one R P (observe t).
+
+Lemma mono_inftaus_ {R} : monotone1 (@inftaus_ R).
+Proof.
+  red; intros. red. destruct IN. eauto.
+Qed.
+Hint Resolve mono_inftaus_ : paco.
+
+Definition inftaus {R} t := paco1 (@inftaus_ R) bot1 t.
+
+Lemma inftaus_or_fintaus {R} (t: itree E R) :
+  inftaus t \/ exists t', unalltaus t t'.
+Proof.
+  destruct (classic (exists t', unalltaus t t')); eauto.
+  left. revert t H. pcofix CIH.
+  intros. pstep. red. destruct (observe t) eqn:EQ.
+  - exfalso. apply H0. eexists. rewrite EQ. eauto.
+  - econstructor; eauto. right. apply CIH.
+    intros [t' [UNT NOT]]. apply H0.
+    exists t'. eauto.
+  - exfalso. apply H0. eexists. rewrite EQ. eauto.
+Qed.
+
+Lemma eutt_inf_not_fin {R1 R2 RR} t1 t2 t3
+      (REL: @eutt E R1 R2 RR t1 t2)
+      (INF: inftaus t1)
+      (UNA: unalltaus t2 t3):
+  False.
+Proof.
+  destruct UNA as [UNT NOT]. punfold REL. red in REL.
+  punfold INF. red in INF.
+  hinduction UNT before RR; intros.
+  - hinduction REL before RR; intros; inv INF; eauto.
+    eapply IHREL; eauto.
+    pclearbot. punfold BASE.
+  - subst. eapply IHUNT; eauto.
+    pstep_reverse. eapply eqit_inv_tauR.
+    pstep. apply REL.
+Qed.
+
+End EUTT_inftaus.
+
+Hint Constructors taus_one.
+Hint Resolve mono_inftaus_ : paco.
+
+Lemma eutt_inv {E R1 R2 RR} t1 t2 (P: _ -> _ -> Prop)
+      (INF: forall ot1 ot2 (INF1: inftaus (go ot1)) (INF2: inftaus (go ot2)), P ot1 ot2)
+      (RET: forall r1 r2
+               (IN: RR r1 r2 : Prop),
+          P (RetF r1) (RetF r2))
+      (VIS: forall u e k1 k2
+               (IN: forall x : u, eutt RR (k1 x) (k2 x)),
+            P (VisF e k1) (VisF e k2))
+      (TAUL: forall t1 ot2 (EQV: eutt RR t1 (go ot2)) (IN: P (observe t1) ot2),
+             P (TauF t1) ot2)
+      (TAUR: forall ot1 t2 (EQV: eutt RR (go ot1) t2) (IN: P ot1 (observe t2)),
+             P ot1 (TauF t2)):
+  @eutt E R1 R2 RR t1 t2 -> P (observe t1) (observe t2).
+Proof.
+  intros. subst.
+  destruct (inftaus_or_fintaus t1) as [INF1 | FIN1], (inftaus_or_fintaus t2) as [INF2 | FIN2]; eauto.
+  - eapply INF.
+    + pstep. punfold INF1.
+    + pstep. punfold INF2.
+  - destruct FIN2. exfalso. eapply eutt_inf_not_fin; eauto.
+  - destruct FIN1. exfalso. apply eqit_flip in H.
+    eapply eutt_inf_not_fin; eauto.
+  - destruct FIN1 as [t1' [UNT1 NOT1]], FIN2 as [t2' [UNT2 NOT2]].
+    punfold H. red in H. simpl in *.
+    hinduction UNT1 before TAUR; intros.
+    + hinduction UNT2 before TAUR; intros.
+      * inv H; try contradiction; eauto.
+        eapply VIS. intros. pclearbot. edestruct (REL x); eauto.
+      * subst. inv H; try contradiction.
+        eapply TAUR; eauto.
+    + subst. eapply TAUL; eauto.
+      * eapply eqit_inv_tauL. pstep. apply H.
+      * eapply IHUNT1; eauto. pstep_reverse.
+        eapply eqit_inv_tauL. pstep. apply H.
+Qed.
+
+Lemma simpobs {E R} {ot} {t: itree E R} (EQ: ot = observe t): t ≅ go ot.
+Proof.
+  pstep. repeat red. simpobs. simpl. subst. pstep_reverse. apply Reflexive_eqit.
+Qed.
+
+Lemma eqit_trans {E R} b (t1 t2 t3: itree E R)
+      (REL1: eqit eq b false bot2 t1 t2)
+      (REL2: eqit eq b false bot2 t2 t3):
+  eqit eq b false bot2 t1 t3.
+Proof.
+  ginit. guclo eqit_clo_trans; eauto.
+  econstructor; eauto with paco. reflexivity.
+Qed.
+
+Lemma eutt_trans {E R} (t1 t2 t3: itree E R)
+      (REL1: t1 ≈ t2)
+      (REL2: t2 ≈ t3):
+  t1 ≈ t3.
+Proof.
+  revert_until R. pcofix CIH; intros.
+  punfold REL1. red in REL1. punfold REL2. red in REL2. pstep. red.
+  hinduction REL1 before CIH; clear t1 t2; intros; subst.
+  - remember (RetF r2) as ot.
+    hinduction REL2 before CIH; intros; subst; try inv Heqot; eauto.
+  - remember (TauF m2) as ot.
+    hinduction REL2 before CIH; intros; subst; try inv Heqot; pclearbot; eauto.
+    econstructor; eauto.
+    rewrite (itree_eta' ot2) in REL2. punfold_reverse REL2.
+    rewrite (itree_eta' ot2). pstep_reverse.
+Admitted.
+      
 Section EUTT_REL.
 
-Context {T1 T2 : Type}.
+(* Context {T1 T2 : Type}. *)
+(* This is for making "rpair bot2 bo2" type-checked *)
+Context {E : Type -> Type} {R1 R2 : Type}.
+Local Notation T1 := (itree E R1).  
+Local Notation T2 := (itree E R2).
 
 Definition eutt_rel := (T1 * T2) + (T1 * T2) -> Prop.
 
@@ -87,79 +234,436 @@ Proof.
   intros. destruct x0, p; contradiction.
 Qed.
 
+Lemma rpair_union r1 r2 r3 r4:
+  (rpair r1 r2 \1/ rpair r3 r4) <1= rpair (r1 \2/ r3) (r2 \2/ r4).
+Proof.
+  intros. destruct PR; eapply rpair_mon; eauto.
+Qed.
+
 End EUTT_REL.
 
 Hint Unfold rpair rfst rsnd.
 Hint Resolve rpair_mon rfst_mon rsnd_mon : paco.
-     
+
+
 Section EUTTG.
 
 Context {E : Type -> Type} {R1 R2 : Type} (RR : R1 -> R2 -> Prop).
 
 Definition euttG_ (rp: eutt_rel) : eutt_rel :=
-  rpair (@eqit_ E _ _ RR true true (rsnd rp) (rfst rp))
-        (eqit_trans_clo true true true true (rfst rp)).
+  rpair (eqit_trans_clo true true true true (rsnd rp))
+        (@eqit_ E _ _ RR true true (rfst rp) (rsnd rp)).
 
-Definition euttC_trans rp :=
-  rpair (@eqit_trans_clo E R1 R2 true true false false (rfst rp))
-        (eqit_trans_clo true true true true (rsnd rp)).
+Definition euttG_transH := @eqit_trans_clo E R1 R2 true true true true.
+Definition euttG_transL := @eqit_trans_clo E R1 R2 true true false false.
+Definition euttG_trans rp := rpair (euttG_transH (rfst rp)) (euttG_transL (rsnd rp)).
 
-Definition euttC_bind rp :=
+Definition euttG_bind rp :=
   rpair (@eqit_bind_clo E R1 R2 true true (rfst rp))
         (eqit_bind_clo true true (rsnd rp)).
-  
-Definition euttC := euttC_trans \2/ euttC_bind.
 
-Definition euttG lp hp := gpaco1 euttG_ euttC lp hp.
+Definition euttC := euttG_trans.
+Definition euttP rH rL gL gH :=
+  gpaco1 euttG_ euttC
+         (rpair (euttG_transH rH)
+                (euttG_transH rH \2/ euttG_transL rL))
+         (rpair (euttG_transH rH \2/ euttG_transL rL \2/ euttG_transL gL \2/ euttG_transH gH)
+                (euttG_transH rH \2/ euttG_transL rL \2/ euttG_transL gL)).
 
-Definition euttL r rl rh := rfst (euttG (rpair r r) (rpair rl rh)).
+Definition euttG rH rL gL gH := rsnd (euttP rH rL gL gH).
 
-Definition euttH r rh := rsnd (euttG (rpair r r) (rpair r rh)).
+Definition euttH rH rL gL gH := rfst (euttP rH rL gL gH).
+
+Hint Unfold euttG_ euttG_transH euttG_transL euttG_trans euttG_bind euttC euttP euttG.
 
 Lemma euttG__mon: monotone1 euttG_.
 Proof.
   red; intros. destruct x0, p; simpl in *.
+  - destruct IN; eauto.  
   - eapply eqitF_mono; eauto.
-  - destruct IN; eauto.
 Qed.
 
 Hint Resolve euttG__mon : paco.
 
-Lemma euttC_trans_wcompat: wcompatible1 euttG_ euttC_trans.
+Lemma euttG_trans_wcompat: wcompatible1 euttG_ euttG_trans.
 Proof.
   econstructor.
   { red; intros. destruct x0, p; simpl in *; destruct IN; eauto. }
-  intros.
-  admit.
-Admitted.
-
-Lemma euttC_bind_wcompat: wcompatible1 euttG_ euttC_bind.
-Proof.
-  econstructor.
-  { red; intros. destruct x0, p; simpl in *; destruct IN; eauto with paco. }
-  intros.
-  admit.
-Admitted.
+  intros. destruct x0, p.
+  { destruct PR. inv RELATED.
+    econstructor.
+    - eapply eutt_trans; eauto.
+    - eapply eutt_trans; eauto.
+    - gbase. eauto.
+  }
+  { destruct PR. punfold EQVl. punfold EQVr. unfold_eqit. repeat red.
+    hinduction RELATED before r; intros; clear t1' t2'.
+    - remember (RetF r1) as x.
+      hinduction EQVl before r; intros; subst; try inv Heqx; eauto.
+      remember (RetF r3) as y.
+      hinduction EQVr before r; intros; subst; try inv Heqy; eauto.
+    - remember (TauF m1) as x.
+      hinduction EQVl before r; intros; subst; try inv Heqx; try inv CHECK; eauto.
+      remember (TauF m3) as y.
+      hinduction EQVr before r; intros; subst; try inv Heqy; try inv CHECK; eauto.
+      pclearbot. econstructor. gclo.
+      econstructor; cycle -1; eauto with paco.
+    - remember (VisF e k1) as x.
+      hinduction EQVl before r; intros; subst; try dependent destruction Heqx; try inv CHECK; eauto.
+      remember (VisF e0 k3) as y.
+      hinduction EQVr before r; intros; subst; try dependent destruction Heqy; try inv CHECK; eauto.
+      econstructor. intros. pclearbot.
+      destruct (REL1 v).
+      + left. gclo. econstructor; eauto with paco.
+      + right. gclo. econstructor; eauto with paco.
+        * eapply eqit_mon, REL0; eauto.
+        * eapply eqit_mon, REL; eauto.
+    - remember (TauF t1) as x.
+      hinduction EQVl before r; intros; subst; try inv Heqx; try inv CHECK; eauto.
+      pclearbot. punfold REL.
+    - remember (TauF t2) as y.
+      hinduction EQVr before r; intros; subst; try inv Heqy; try inv CHECK; eauto.
+      pclearbot. punfold REL.
+  }
+Qed.
 
 Lemma euttC_wcompat: wcompatible1 euttG_ euttC.
 Proof.
-  apply wcompat1_union; eauto with paco.
-  - apply euttC_trans_wcompat.
-  - apply euttC_bind_wcompat.
+  apply euttG_trans_wcompat.
 Qed.
+
+Lemma euttG_clo_trans: euttG_trans <2= gupaco1 euttG_ euttC.
+Proof.
+  intros. gclo. destruct x1, p; destruct PR; econstructor; eauto with paco.
+Qed.  
+
+Lemma euttG_clo_bind: euttG_bind <2= gupaco1 euttG_ euttC.
+Proof.
+  gcofix CIH. intros. destruct x2, p.
+  - inv PR. gclo. econstructor.
+    { rewrite (itree_eta t1); reflexivity. }
+    { rewrite (itree_eta t2); reflexivity. }
+    move EQV before RU. revert_until EQV.
+    eapply (eutt_inv t1 t2), EQV; intros.
+    + gstep. econstructor; try reflexivity.
+      clear - INF1 INF2. revert_until ot2. generalize (go ot1) (go ot2). clear ot1 ot2.
+      gcofix CIH. intros.
+      punfold INF1. inv INF1. punfold INF2. inv INF2. pclearbot.
+      gstep. repeat red. rewrite !unfold_bind. simpobs. simpl. eauto with paco.
+    + gclo. econstructor.
+      * rewrite bind_ret_. reflexivity.
+      * rewrite bind_ret_. reflexivity.
+      * gbase. eapply REL. eauto.
+    + gstep. econstructor.
+      * rewrite bind_vis_. reflexivity.
+      * rewrite bind_vis_. reflexivity.
+      * gstep. econstructor. right.
+        gbase. eapply CIH. econstructor; [apply IN|eauto].
+    + gclo. econstructor; [|reflexivity|eauto].
+      rewrite bind_tau_, <-itree_eta. apply eqit_tauL. reflexivity.
+    + gclo. econstructor; [reflexivity| |eauto].
+      rewrite bind_tau_, <-itree_eta. apply eqit_tauL. reflexivity.
+  - destruct PR. punfold EQV. red in EQV.
+    genobs t1 ot1. genobs t2 ot2.
+    hinduction EQV before RU; intros; subst; pclearbot.
+    + gclo. econstructor; cycle -1.
+      * gbase. eapply REL0. apply REL.
+      * rewrite (simpobs Heqot1), bind_ret_. reflexivity.
+      * rewrite (simpobs Heqot2), bind_ret_. reflexivity.
+    + gstep. repeat red. rewrite !unfold_bind. simpobs. simpl.
+      econstructor. gbase. eapply CIH.
+      econstructor; eauto.
+    + gstep. repeat red. rewrite !unfold_bind. simpobs. simpl.
+      econstructor. left. gbase. eapply CIH.
+      econstructor; eauto.
+    + gclo. econstructor; [|reflexivity|eauto].
+      rewrite (simpobs Heqot1), bind_tau_. apply eqit_tauL. reflexivity.
+    + gclo. econstructor; [reflexivity| |eauto].
+      rewrite (simpobs Heqot2), bind_tau_. apply eqit_tauL. reflexivity.
+Qed.
+
+Global Instance eq_euttG r1 r2:
+  Proper (eq_itree eq ==> eq_itree eq ==> flip impl)
+         (rsnd (gpaco1 euttG_ euttC r1 r2)).
+Proof.
+  repeat intro. guclo euttG_clo_trans. econstructor; cycle -1; eauto using eqit_mon.
+Qed.
+
+Lemma rclo_euttC: rclo1 euttC <2= euttC.
+Proof.
+  intros. induction PR.
+  - destruct x1, p; econstructor; try reflexivity; eauto.
+  - destruct x1, p; destruct IN.
+    + apply H in RELATED. destruct RELATED.
+      econstructor; cycle -1; eauto; eapply eutt_trans; eauto.
+    + apply H in RELATED. destruct RELATED.
+      econstructor; cycle -1; eauto; eapply eqit_trans; eauto.
+Qed.
+
+Lemma euttG_inv t1 t2 rH rL gL gH (P: _ -> _ -> Prop)
+      (INF: forall ot1 ot2 (INF1: inftaus (go ot1)) (INF2: inftaus (go ot2)), P ot1 ot2)
+      (BASE: forall t1 t2
+               (IN: (euttG_transH rH \2/ euttG_transL rL) t1 t2 : Prop),
+          P (observe t1) (observe t2))
+      (RET: forall r1 r2
+               (IN: RR r1 r2 : Prop),
+          P (RetF r1) (RetF r2))
+      (VIS: forall u e k1 k2
+               (IN: forall x : u, euttH (rH \2/ rL \2/ gL \2/ gH) (rH \2/ rL \2/ gL \2/ gH) (rH \2/ rL \2/ gL \2/ gH) (rH \2/ rL \2/ gL \2/ gH) (k1 x) (k2 x)),
+            P (VisF e k1) (VisF e k2))
+      (TAUL: forall t1 ot2 (IN: P (observe t1) ot2),
+             P (TauF t1) ot2)
+      (TAUR: forall ot1 t2 (IN: P ot1 (observe t2)),
+             P ot1 (TauF t2)):
+  euttG rH rL gL gH t1 t2 -> P (observe t1) (observe t2).
+Proof.
+  revert t1 t2; intros.
+  destruct (inftaus_or_fintaus t1) as [INF1 | FIN1], (inftaus_or_fintaus t2) as [INF2 | FIN2]; intros.
+  { eapply INF.
+    - pstep. punfold INF1.
+    - pstep. punfold INF2.
+  }
+  { destruct FIN2. inv H0. gunfold H. apply rclo_euttC in H.
+    destruct H. destruct RELATED; cycle 1.
+    + eapply BASE. destruct H, H.
+      * left. econstructor; cycle -1; eauto; eapply eutt_trans; eauto using eqit_mon.
+      * right. econstructor; cycle -1; eauto; eapply eqit_trans; eauto.
+    + repeat red in H.
+
+      punfold EQVl. red in EQVl. punfold EQVr. red in EQVr. 
+        genobs t1' ot1'. genobs t2' ot2'.
+        hinduction H before TAUR; intros; subst; dependent destruction EQVr; simpobs; try inv H2; try discriminate.
+        * exfalso. punfold INF1; red in INF1. remember (RetF r1) as ot.
+          induction EQVl; intros; subst; try inv INF1; try inv Heqot.
+          eapply IHEQVl; eauto. pclearbot. punfold BASE0.
+        * exfalso. punfold INF1; red in INF1. remember (VisF e k1) as ot.
+          induction EQVl; intros; subst; try inv INF1; try inv Heqot.
+          eapply IHEQVl; eauto. pclearbot. punfold BASE0.
+        * eapply (IHeqitF t0 (Ret r2)); simpl; eauto.
+          pstep_reverse. eapply eqit_inv_tauR. pstep. eauto.
+        * eapply (IHeqitF t0 (Vis e k1)); simpl; eauto.
+          pstep_reverse. eapply eqit_inv_tauR. pstep. eauto.
+
+    
+
+
+
+
+
+
+    destruct FIN2. inv H0. genobs t2 ot2. genobs x ox.
+    hinduction H1 before TAUR; intros; subst.
+    - clear x Heqox. gunfold H.
+      apply rclo_euttC in H.
+      destruct H. destruct RELATED; cycle 1.
+      + eapply BASE. destruct H, H.
+        * left. econstructor; cycle -1; eauto; eapply eutt_trans; eauto using eqit_mon.
+        * right. econstructor; cycle -1; eauto; eapply eqit_trans; eauto.
+      + punfold EQVl. red in EQVl. punfold EQVr. red in EQVr. repeat red in H.
+        genobs t1' ot1'. genobs t2' ot2'.
+        hinduction H before TAUR; intros; subst; dependent destruction EQVr; simpobs; try inv H2; try discriminate.
+        * exfalso. punfold INF1; red in INF1. remember (RetF r1) as ot.
+          induction EQVl; intros; subst; try inv INF1; try inv Heqot.
+          eapply IHEQVl; eauto. pclearbot. punfold BASE0.
+        * exfalso. punfold INF1; red in INF1. remember (VisF e k1) as ot.
+          induction EQVl; intros; subst; try inv INF1; try inv Heqot.
+          eapply IHEQVl; eauto. pclearbot. punfold BASE0.
+        * eapply (IHeqitF t0 (Ret r2)); simpl; eauto.
+          pstep_reverse. eapply eqit_inv_tauR. pstep. eauto.
+        * eapply (IHeqitF t0 (Vis e k1)); simpl; eauto.
+          pstep_reverse. eapply eqit_inv_tauR. pstep. eauto.
+    - gunfold H. apply rclo_euttC in H.
+      destruct H. punfold EQVr. red in EQVr. simpobs. rewrite (itree_eta' (TauF t')) in EQVr.
+      punfold_reverse EQVr. eapply eqit_inv_tauL in EQVr.
+      
+
+      
+  }
+  { admit. }
+  admit.
+Admitted.
 
 End EUTTG.
 
+Hint Unfold euttG_ euttG_transH euttG_transL euttG_trans euttG_bind euttC euttP euttG.
 Hint Resolve euttG__mon : paco.
 Hint Resolve euttC_wcompat : paco.
+
+(* Lemma eq_itree_inv_bind {E R1 R2} t1 (s2: itree E R1) (k2: R1 -> itree E R2) *)
+(*       (REL: t1 ≈ (x <- s2;; k2 x)): *)
+(*   exists s1 k1, t1 = (x <- s1;; k1 x) /\ s1 ≈ s2 /\ (forall v, k1 v ≈ k2 v). *)
+(* Proof. *)
+(* Qed. *)
 
 Section EUTTG_Properties.
 
 Context {E : Type -> Type} {R1 R2 : Type} (RR : R1 -> R2 -> Prop).
 
+Local Notation euttP := (@euttP E R1 R2 RR).
 Local Notation euttG := (@euttG E R1 R2 RR).
-Local Notation euttH := (@euttH E R1 R2 RR).
-Local Notation euttL := (@euttH E R1 R2 RR).
+
+(* Lose weak hypotheses after general rewriting *)
+
+Lemma euttG_trans_eutt rH rL gL gH t1 t2:
+  eqit_trans_clo true true true true (euttG rH rH rH gH) t1 t2 -> euttG rH rL gL gH t1 t2.
+Proof.
+  revert t1 t2. gcofix CIH; intros.
+  destruct H0. punfold EQVl; red in EQVl. punfold EQVr; red in EQVr.
+  revert t1 t2 EQVl EQVr.
+  eapply (euttG_inv RR t1' t2'), RELATED; intros.
+  - admit.
+  - gbase. left. destruct IN, H.
+    + econstructor; cycle -1; eauto; eapply eutt_trans; eauto.
+    + econstructor; cycle -1; eauto; eapply eutt_trans; eauto using eqit_mon.
+  - admit.
+  - 
+
+
+  red in RELATED. rewrite (itree_eta t1') in RELATED.
+  change (gpaco1 (euttG_ RR) euttC (rpair gH gL) r (inr (t1, t2)))
+         with (rsnd (gpaco1 (euttG_ RR) euttC (rpair gH gL) r ) t1 t2).
+  rewrite (itree_eta t1).
+  revert t2 t2' EQVr RELATED. eapply (eutt_inv t1 t1'), EQVl; intros.
+  - 
+  
+
+
+  gclo. econstructor.
+  { rewrite itree_eta. reflexivity. }
+  { rewrite itree_eta. reflexivity. }
+  revert t2 t2' EQVr RELATED.
+
+Qed.
+
+
+(* Lemma euttG_trans_euttL rH rL gL gH *)
+(*       (GOOD: eqit_trans_clo true true true true rH <2= rH) *)
+(*       (INV: rH <2= rL /\ rL <2= gL /\ gL <2= gH): *)
+(*   forall t1 t0 t2 *)
+(*       (EQVl: eqit eq true true bot2 t1 t0) *)
+(*       (REL: euttG rH rH rH gH t0 t2), *)
+(*   euttG rH rL gL gH t1 t2. *)
+(* Proof. *)
+(*   gcofix CIH. intros. *)
+(*   punfold EQVl. red in EQVl. genobs t1 ot1. genobs t0 ot0. *)
+(*   hinduction EQVl before CIH; intros; subst. *)
+(*   - gunfold REL0. remember (inl (t0, t2)) as x. *)
+(*     hinduction REL0 before CIH; intros; subst. *)
+(*     + destruct IN. *)
+(*       * gstep.  repeat red in H. repeat red. *)
+(*         hinduction H before CIH; intros; inv Heqot0; simpobs; eauto. *)
+(*         econstructor; eauto. eapply (IHeqitF r2 (Ret r2)); eauto. *)
+(*       * gbase. apply INV. simpl in H. *)
+(*         eapply GOOD. econstructor; eauto; try reflexivity. *)
+(*         rewrite (itree_eta t1), (itree_eta t0). simpobs. reflexivity. *)
+(*     + destruct IN. *)
+(*       * destruct H0. gclo. left. econstructor; cycle -1. *)
+(*         -- eapply H; [eauto|..|eauto]. *)
+(*         -- *)
+(*          punfold EQVl. red in EQVl. simpobs. *)
+(*         -- punfold EQVl. *)
+(*         (* eapply H; [eauto|..]. *) admit. *)
+(*       * admit. *)
+(*   - *)
+(* Qed. *)
+
+(* Lemma foo rL rH: *)
+(*   @eqit_trans_clo E R1 R2 true true true true (rsnd (rclo1 euttC (rpair rH rL))) *)
+(*   <2= rsnd (rclo1 euttC (rpair rH (eqit_trans_clo true true true true rL))). *)
+(* Proof. *)
+(*   intros. destruct PR. repeat red in RELATED. remember (inr (t1', t2')) as x. *)
+(*   hinduction RELATED before rH; intros; subst. *)
+(*   - apply rclo1_base. eauto. *)
+(*   - destruct IN. apply rclo1_clo. *)
+(*     econstructor; [| |eapply H; [eauto|..|eauto]]. *)
+(*     + reflexivity. *)
+(*     + reflexivity. *)
+(*     + eapply eutt_trans; eauto. *)
+(*       eapply eqit_mon, EQVl0; eauto. *)
+(*     + eapply eutt_trans; eauto. *)
+(*       eapply eqit_mon, EQVr0; eauto. *)
+(* Qed. *)
+
+
+
+Lemma euttG_trans_eutt rH rL gL gH
+      (INV: rH <2= rL /\ rL <2= gL /\ gL <2= gH)
+      (GOOD: eqit_trans_clo true true true true rH <2= rH) t1 t2:
+  eqit_trans_clo true true true true (euttG rH rH rH gH) t1 t2 -> euttG rH rL gL gH t1 t2.
+Proof.
+  intros. destruct H. gunfold RELATED.
+  hexploit foo; [econstructor; [apply EQVl|apply EQVr|..]|].
+  { eapply rclo1_mon; [apply RELATED|]. intros. apply rpair_union, PR. }
+  intros IN.
+  econstructor. red in IN.
+  cut (eqit_trans_clo true true true true (eqit_ RR true true
+         (rsnd (gupaco1 (euttG_ RR) euttC (rpair rH gH \1/ rpair rH rH)))
+         (rfst (gupaco1 (euttG_ RR) euttC (rpair rH gH \1/ rpair rH rH))) \2/ rH)
+       <2= rfst (paco1 (euttG_ RR ∘ rclo1 euttC) (rpair gL gH \1/ rpair rL rH) \1/ rpair rL rH)).
+  { admit. }
+
+  intros. red. destruct PR. destruct RELATED0; cycle 1.
+  { right. eapply INV. eauto. }
+  left. red in H.
+  
+  
+
+  eapply rclo1_mon. apply IN.
+  intros. destruct x0, p; simpl in *.
+  - 
+
+  
+
+  
+Qed.
+
+  
+
+
+(* Make new hypotheses *)
+
+Lemma euttG_coind: forall rH rL gL gH (INV: rH <2= rL /\ rL <2= gL /\ gL <2= gH) x,
+    (x <2= euttG rH rL (gL \2/ x) (gH \2/ x)) -> (x <2= euttG rH rL gL gH).
+
+(* Process itrees *)
+
+Lemma euttG_ret: forall rH rL gL gH (INV: rH <2= rL /\ rL <2= gL /\ gL <2= gH) v1 v2,
+  RR v1 v2 -> euttG rH rL gL gH (Ret v1) (Ret v2).
+
+Lemma euttG_bind: forall rH rL gL gH (INV: rH <2= rL /\ rL <2= gL /\ gL <2= gH) t1 t2,
+  eqit_bind_clo true true (euttG rH rL gL gH) t1 t2 -> euttG rH rL gL gH t1 t2.
+
+Lemma euttG_trans_eq: forall rH rL gL gH (INV: rH <2= rL /\ rL <2= gL /\ gL <2= gH) t1 t2,
+  eqit_trans_clo true true false false (euttG rH rL gL gH) t1 t2 -> euttG rH rL gL gH t1 t2.
+
+
+(* Make available weak hypotheses *)
+
+Lemma euttG_tau: forall rH rL gL gH (INV: rH <2= rL /\ rL <2= gL /\ gL <2= gH) t1 t2,
+  euttG rH gL gL gH t1 t2 -> euttG rH rL gL gH (Tau t1) (Tau t2).
+
+(* Make available strong hypotheses *)
+
+Lemma euttG_vis: forall rH rL gL gH (INV: rH <2= rL /\ rL <2= gL /\ gL <2= gH) u (e: E u) k1 k2,
+  (forall v, euttG gH gH gH gH (k1 v) (k2 v)) -> euttG rH rL gL gH (Vis e k1) (Vis e k2).
+
+(* Use available hypotheses *)
+
+Lemma euttG_base: forall rH rL gL gH (INV: rH <2= rL /\ rL <2= gL /\ gL <2= gH) t1 t2,
+  rL t1 t2 -> euttG rH rL gL gH t1 t2.
+
+
+
+
+
+
+
+
+
+
+
+
+
 
 Lemma rclo1_euttC_mon_fst r r'
       (LE: rfst r <2= rsnd r'):
@@ -185,9 +689,27 @@ Proof.
     + apply rclo1_clo. right. destruct H0. unfold rsnd in *. econstructor; eauto.
 Qed.
 
+(* Lemma foo rh: *)
+(*    euttG (rpair rh rh) (rpair rh rh) <1= *)
+(*    euttG (rpair (rsnd (euttG (rpair bot2 rh) (rpair bot2 rh))) rh) *)
+(*          (rpair (rsnd (euttG (rpair bot2 rh) (rpair bot2 rh))) rh). *)
+(* Proof. *)
+(*   gcofix CIH. intros. *)
+(*   destruct x1, p. *)
+(*   - gunfold PR. gupaco. econstructor. *)
+(*     eapply rclo1_euttC_mon_snd, IN. clear t1 t2 IN. *)
+(*   intros. destruct PR; right; cycle 1. *)
+(*   { gbase. apply H. } *)
+(*   gclo. left. destruct H. econstructor; eauto. clear t1 t2 EQVl EQVr. *)
+(*   red in RELATED. red.  *)
+(* Qed. *)
+
+
+
+
 Lemma foo rh t1 t2
       (IN: euttH rh rh t1 t2) :
-  rsnd (euttG (rpair (@bot2 _ (fun _ => _)) rh) (rpair (@bot2 _ (fun _ => _)) rh)) t1 t2.
+  rsnd (euttG (rpair bot2 rh) (rpair bot2 rh)) t1 t2.
 Proof.
   revert t1 t2 IN. gcofix CIH. intros.
   gunfold IN. gupaco. econstructor.
@@ -195,8 +717,15 @@ Proof.
   intros. destruct PR; right; cycle 1.
   { gbase. apply H. }
   gclo. left. destruct H. econstructor; eauto. clear t1 t2 EQVl EQVr.
+  red in RELATED. red. 
+  
 
-  red in RELATED.
+  
+
+
+  
+  revert t1' t2' RELATED. gcofix CIH.
+
 
 
   
@@ -243,7 +772,79 @@ Proof.
 Qed.
 
 
-  
+
+
+
+
+
+
+
+
+
+
+
+Section Test.
+
+Context {E : Type -> Type} {R1 R2 : Type} (RR : R1 -> R2 -> Prop).
+
+Variable euttG: forall (rH rL gL gH : itree E R1 -> itree E R2 -> Prop), itree E R1 -> itree E R2 -> Prop.
+
+(**
+   Correctness
+ **)
+
+Axiom eutt_le_euttG:
+  eutt RR <2= euttG bot2 bot2 bot2 bot2.
+
+Axiom euttG_le_eutt:
+  euttG bot2 bot2 bot2 bot2 <2= eutt RR.
+
+(**
+   Reasoning Principles
+ **)
+
+(* Make new hypotheses *)
+
+Axiom euttG_coind: forall rH rL gL gH (INV: rH <2= rL /\ rL <2= gL /\ gL <2= gH) x,
+  (x <2= euttG rH rL (gL \2/ x) (gH \2/ x)) -> (x <2= euttG rH rL gL gH).
+
+(* Process itrees *)
+
+Axiom euttG_ret: forall rH rL gL gH (INV: rH <2= rL /\ rL <2= gL /\ gL <2= gH) v1 v2,
+  RR v1 v2 -> euttG rH rL gL gH (Ret v1) (Ret v2).
+
+Axiom euttG_bind: forall rH rL gL gH (INV: rH <2= rL /\ rL <2= gL /\ gL <2= gH) t1 t2,
+  eqit_bind_clo true true (euttG rH rL gL gH) t1 t2 -> euttG rH rL gL gH t1 t2.
+
+Axiom euttG_trans_eq: forall rH rL gL gH (INV: rH <2= rL /\ rL <2= gL /\ gL <2= gH) t1 t2,
+  eqit_trans_clo true true false false (euttG rH rL gL gH) t1 t2 -> euttG rH rL gL gH t1 t2.
+
+(* Lose weak hypotheses after general rewriting *)
+
+Axiom euttG_trans_eutt: forall rH rL gL gH (INV: rH <2= rL /\ rL <2= gL /\ gL <2= gH) t1 t2,
+  eqit_trans_clo true true true true (euttG rH rH rH gH) t1 t2 -> euttG rH rL gL gH t1 t2.
+
+(* Make available weak hypotheses *)
+
+Axiom euttG_tau: forall rH rL gL gH (INV: rH <2= rL /\ rL <2= gL /\ gL <2= gH) t1 t2,
+  euttG rH gL gL gH t1 t2 -> euttG rH rL gL gH (Tau t1) (Tau t2).
+
+(* Make available strong hypotheses *)
+
+Axiom euttG_vis: forall rH rL gL gH (INV: rH <2= rL /\ rL <2= gL /\ gL <2= gH) u (e: E u) k1 k2,
+  (forall v, euttG gH gH gH gH (k1 v) (k2 v)) -> euttG rH rL gL gH (Vis e k1) (Vis e k2).
+
+(* Use available hypotheses *)
+
+Axiom euttG_base: forall rH rL gL gH (INV: rH <2= rL /\ rL <2= gL /\ gL <2= gH) t1 t2,
+  rL t1 t2 -> euttG rH rL gL gH t1 t2.
+
+End Test.
+
+
+
+
+
 
 (**
    Correctness
@@ -332,6 +933,8 @@ Axiom euttL_higher: forall r rl rh (INV: r <2= rl /\ rl <2= rh) u (e: E u) k1 k2
 
 
 End EUTTG_Properties.
+
+
 
 
 
